Remove more complicated proof from decode_pk for stability's sake
Since we have to assume the output of decode_pk is valid, remove the more
fine-grained proof that was there which would have been used had we been
able to prove the operations actually guaranteed the bounds. Since it turns
out that's not the case, remove all the proof code around slowly expanding
a public key to satisfy the predicate, and just assume the whole thing is
in range with an assumption at the end.

The proof had been assuming the smallest possible fact and then using that
to build to the larger conclusion, but that was making the prover randomly
cancel.

qtesla/code/Hacl.Impl.QTesla.Heuristic.Pack.fst
@@ -280,14 +280,6 @@ let decode_pk_set_pk snapshot pk_in pk i j value =
     assert(forall (k:nat{k < 32}) (h:HS.mem) . {:pattern bget h pk (v i + k) \/ bget h (gsub pk i (size 32)) k} bget h pk (v i + k) == bget h (gsub pk i (size 32)) k);
     reveal_valid_decode_pk pk_in pk snapshot h1 i
 
-private let lemma_decode_pk_extend 
-    (pk : lbuffer I32.t (params_n *. params_k))
-    (i : size_t{v i + 31 < v params_n * v params_k})
-    (h : HS.mem) : Lemma
-    (requires is_poly_k_pk_i h pk (v i) /\
-              (forall (k:nat{k >= v i /\ k < v i + 32}) . is_pk (bget h pk k)))
-    (ensures is_poly_pk_i h pk (v i + 32)) = ()
-
 private inline_for_extraction noextract
 val decode_pk_loopBody:
     pk : lbuffer I32.t (params_n *. params_k)
@@ -296,14 +288,14 @@ val decode_pk_loopBody:
   -> i : size_t{v i + 31 < v params_n * v params_k}
   -> j : size_t{v j + 22 < v crypto_publickeybytes / 4}
   -> Stack unit
-    (requires fun h -> live h pk /\ live h pk_in /\ disjoint pk pk_in /\ is_poly_k_pk_i h pk (v i))
-    (ensures fun h0 _ h1 -> modifies1 pk h0 h1 /\ is_poly_k_pk_i h1 pk (v i + 32))
+    (requires fun h -> live h pk /\ live h pk_in /\ disjoint pk pk_in)
+    (ensures fun h0 _ h1 -> modifies1 (gsub pk i (size 32)) h0 h1)
 
-#push-options "--z3rlimit 1500"
+#push-options "--z3rlimit 800"
 let decode_pk_loopBody pk pk_in mask23 i j =
     let h0 = ST.get () in
     reveal_valid_decode_pk pk_in pk h0 h0 i;
-    //assert(modifies1 (gsub pk i (size 32)) h0 h0); 
+    assert(modifies1 (gsub pk i (size 32)) h0 h0); 
     assert(valid_decode_pk pk_in pk h0 h0 i);
 
     // In the reference code, "pt = (uint32_t*)pk_in" where pk_in is (unsigned char *). We can't recast buffers to have
@@ -358,19 +350,7 @@ let decode_pk_loopBody pk pk_in mask23 i j =
 
     let h1 = ST.get () in
     reveal_valid_decode_pk pk_in pk h0 h1 i;
-    assert(valid_decode_pk pk_in pk h0 h1 i); 
-    //assert(modifies1 (gsub pk i (size 32)) h0 h1);
-    assert(forall (k:nat{k < v i}) . bget h0 (gsub pk (size 0) i) k == bget h1 (gsub pk (size 0) i) k); 
-    // ASSUMPTION per Patrick: The above unpacking does not guarantee the values of the coefficients are less than q.
-    // The reference code specifically assumes input public keys are valid, and so we assume this here.
-    assume(forall (k:nat{k >= v i /\ k < v i + 32}) . is_pk (bget h1 pk k));
-    // index reassignment assertion
-    assert(forall (k:nat{k < v i}) (h:HS.mem) . {:pattern bget h pk k \/ bget h (gsub pk (size 0) i) k} bget h pk k == bget h (gsub pk (size 0) i) k); 
-    assert(is_poly_k_pk_i h1 pk (v i)); 
-    // TODO (kkane): This function checks in the interactive mode, but without this admit here, always fails due to being
-    // canceled when run from the command line. Leaving this here for now until we can look into this.
-    admit();
-    lemma_decode_pk_extend pk i h1
+    assert(valid_decode_pk pk_in pk h0 h1 i)
 #pop-options
 
 #push-options "--max_fuel 0"
@@ -389,8 +369,6 @@ val decode_pk:
     (ensures fun h0 _ h1 -> modifies2 pk seedA h0 h1 /\ is_poly_k_pk h1 pk)
 
 let decode_pk pk seedA pk_in =
-    //let iBuf = create (size 1) (size 0) in
-    //let jBuf = create (size 1) (size 0) in
     // In the reference implementation, pp is a uint32_t view into pk. We can't do that in F*, so we operate
     // directly on pk, doing a cast from int32 to uint32 in-line. pt is a uint32_t view into pk, and the
     // function pt above takes care of doing that conversion.
@@ -400,7 +378,7 @@ let decode_pk pk seedA pk_in =
 
     let h0 = ST.get () in
     for (size 0) (params_n /. size 32)
-    (fun h k -> live h pk /\ live h pk_in /\ modifies1 pk h0 h /\ k <= v params_n / 32 /\ is_poly_k_pk_i h pk (k * 32))
+    (fun h k -> live h pk /\ live h pk_in /\ modifies1 pk h0 h)
     (fun k ->
         let j = k *. size 23 in
         let i = k *. size 32 in
@@ -408,12 +386,15 @@ let decode_pk pk seedA pk_in =
         decode_pk_loopBody pk pk_in mask23 i j
     );
 
-    // Actually have to point this fact out to the prover to prove the post-condition.
-    let h1 = ST.get () in
-    assert(is_poly_k_pk_i h1 pk (v (params_n /. size 32) * 32));
-
     assert(v params_k = 1);
-    copy seedA (sub pk_in (params_n *. params_q_log /. size 8) crypto_seedbytes)
+    copy seedA (sub pk_in (params_n *. params_q_log /. size 8) crypto_seedbytes);
+
+    // ASSUMPTION per Patrick: The above unpacking does not guarantee the values of the coefficients are less than q.
+    // The reference code specifically assumes input public keys are valid, and so we assume this here. This isn't a
+    // security vulnerability because "malicious" public keys with coefficients >= q won't actually verify anything
+    // useful.
+    let h1 = ST.get () in
+    assume(is_poly_k_pk h1 pk)
 
 [@"opaque_to_smt"]
 private let valid_encode_sig (z: poly) (sm: lbuffer uint8 crypto_bytes) (h0 h1: HS.mem) =
